proof/drefine/Finalise_DR.thy
@@ -829,7 +829,7 @@ lemma flush_table_exec:
 
 
 lemma transform_cap_not_new_invented:
-  "transform_cap z \<noteq> cdl_cap.PageTableCap word Fake asid"
+  "transform_cap z \<noteq> cdl_cap.PageTableCap word (Fake attr) asid"
   by (auto simp:transform_cap_def split:arch_cap.splits cap.splits)
 
 lemma page_table_not_idle:
@@ -921,7 +921,7 @@ where "pt_page_relation pt page offset S s \<equiv>
 lemma slot_with_pt_frame_relation:
   "\<lbrakk>valid_idle s;pt_page_relation a oid y S s\<rbrakk>\<Longrightarrow>
     (a, nat (uint (y && mask pt_bits >> 2))) \<in>
-    ((slots_with (\<lambda>x. \<exists>rights sz asid. x = FrameCap False oid rights sz Fake asid)) (transform s))"
+    ((slots_with (\<lambda>x. \<exists>attr rights sz asid. x = FrameCap False oid rights sz (Fake attr) asid)) (transform s))"
   apply (clarsimp simp:pt_page_relation_def)
   apply (frule page_table_at_rev)
   apply (frule(1) page_table_not_idle)
@@ -946,7 +946,7 @@ lemma below_kernel_base_int:
 lemma slot_with_pd_pt_relation:
   "\<lbrakk>valid_idle s; pd_pt_relation a b y s; ucast (y && mask pd_bits >> 2) \<notin> kernel_mapping_slots\<rbrakk> \<Longrightarrow>
   (a, unat (y && mask pd_bits >> 2)) \<in>
-    (slots_with (\<lambda>x. \<exists>asid. x = cdl_cap.PageTableCap b Fake asid)) (transform s)"
+    (slots_with (\<lambda>x. \<exists>attr asid. x = cdl_cap.PageTableCap b (Fake attr) asid)) (transform s)"
   apply (clarsimp simp :pd_pt_relation_def)
   apply (frule page_directory_at_rev)
   apply (frule(1) page_directory_not_idle)
@@ -961,7 +961,7 @@ lemma slot_with_pd_section_relation:
   "\<lbrakk>valid_idle s; pd_super_section_relation a b y s \<or> pd_section_relation a b y s;
     ucast (y && mask pd_bits >> 2) \<notin> kernel_mapping_slots\<rbrakk> \<Longrightarrow>
   (a, unat (y && mask pd_bits >> 2)) \<in>
-    (slots_with (\<lambda>x. \<exists>rights sz asid. x = cdl_cap.FrameCap False b rights sz Fake asid)) (transform s)"
+    (slots_with (\<lambda>x. \<exists>attr rights sz asid. x = cdl_cap.FrameCap False b rights sz (Fake attr) asid)) (transform s)"
   apply (erule disjE)
    apply (clarsimp simp :pd_super_section_relation_def)
    apply (frule page_directory_at_rev)
@@ -983,7 +983,7 @@ lemma slot_with_pd_section_relation:
 
 lemma opt_cap_page_table:
   "\<lbrakk> valid_idle s;pd_pt_relation a pt_id x s;ucast (x && mask pd_bits >> 2) \<notin> kernel_mapping_slots \<rbrakk>
-  \<Longrightarrow> opt_cap (a, unat (x && mask pd_bits >> 2)) (transform s) = Some (cdl_cap.PageTableCap pt_id Fake None)"
+  \<Longrightarrow> \<exists>attr. opt_cap (a, unat (x && mask pd_bits >> 2)) (transform s) = Some (cdl_cap.PageTableCap pt_id (Fake attr) None)"
   apply (clarsimp simp :pd_pt_relation_def opt_cap_def transform_def slots_of_def)
   apply (frule page_directory_at_rev)
   apply (frule(1) page_directory_not_idle)
@@ -994,25 +994,24 @@ lemma opt_cap_page_table:
   apply (simp add: mask_pd_bits_less )
   done
 
-lemma opt_cap_page:"\<lbrakk>valid_idle s;pt_page_relation a pg x S s \<rbrakk>\<Longrightarrow>
-\<exists>f sz. (opt_cap (a, unat (x && mask pt_bits >> 2) ) (transform s))
-  = Some (cdl_cap.FrameCap False pg f sz Fake None)"
-  apply (clarsimp simp: pt_page_relation_def opt_cap_def transform_def slots_of_def)
-  apply (frule page_table_at_rev)
-  apply (frule(1) page_table_not_idle)
-  apply (clarsimp simp: transform_objects_def not_idle_thread_def page_directory_not_idle
-                        restrict_map_def object_slots_def)
-  apply (clarsimp simp: transform_page_table_contents_def unat_map_def split:ARM_A.pte.split_asm | rule conjI )+
-    apply (clarsimp simp: transform_page_table_contents_def unat_map_def transform_pte_def)
-   apply (simp add: mask_pt_bits_less)+
-  apply (clarsimp simp: transform_page_table_contents_def unat_map_def transform_pte_def)
+lemma opt_cap_page:
+  "\<lbrakk> valid_idle s; pt_page_relation a pg x S s \<rbrakk>\<Longrightarrow>
+   \<exists>attr f sz. opt_cap (a, unat (x && mask pt_bits >> 2)) (transform s) =
+                 Some (cdl_cap.FrameCap False pg f sz (Fake attr) None)"
+  unfolding pt_page_relation_def transform_def opt_cap_def slots_of_def
+  apply clarsimp
+  apply (frule transform_objects_kheap)
+   apply (fastforce dest!: arch_obj_not_idle simp: not_idle_thread_def)
+  apply (fastforce simp: object_slots_def transform_page_table_contents_def unat_map_def
+                         transform_pte_def mask_pt_bits_less
+                   split: ARM_A.pte.split_asm)
   done
 
 lemma opt_cap_section:
   "\<lbrakk>valid_idle s;pd_section_relation a pg x s \<or> pd_super_section_relation a pg x s;
     ucast (x && mask pd_bits >> 2) \<notin> kernel_mapping_slots\<rbrakk>\<Longrightarrow>
-  \<exists>f sz. (opt_cap (a, unat (x && mask pd_bits >> 2) ) (transform s))
-    = Some (cdl_cap.FrameCap False pg f sz Fake None)"
+  \<exists>attr f sz. (opt_cap (a, unat (x && mask pd_bits >> 2) ) (transform s))
+    = Some (cdl_cap.FrameCap False pg f sz (Fake attr) None)"
   apply (erule disjE)
    apply (clarsimp simp: pd_section_relation_def opt_cap_def transform_def slots_of_def)
    apply (frule page_directory_at_rev)
