spec/capDL/ARM/Arch_Structs_D.thy
@@ -1,0 +1,32 @@
+(*
+ * Copyright 2020, Data61, CSIRO (ABN 41 687 119 230)
+ *
+ * SPDX-License-Identifier: GPL-2.0-only
+ *)
+
+theory Arch_Structs_D
+imports
+  ExecSpec.MachineTypes
+begin
+
+context Arch begin global_naming ARM_D
+
+(* Sizes are duplicated from ARM ASpec and must be kept in sync *)
+
+definition slot_bits_cdl :: nat where
+  "slot_bits_cdl \<equiv> 4"
+
+definition endpoint_bits_cdl :: nat where
+  "endpoint_bits_cdl \<equiv> 4"
+
+definition tcb_bits_cdl :: nat where
+  "tcb_bits_cdl \<equiv> 9"
+
+definition ntfn_bits_cdl :: nat where
+  "ntfn_bits_cdl \<equiv> 4"
+
+definition pageBits_cdl :: "nat" where
+  "pageBits_cdl \<equiv> smallPageBits"
+
+end
+end
